examples/mutsum/MutF01proof.v
@@ -48,20 +48,20 @@ Section SIMMODSEM.
     i. eapply adequacy_lift.
     econstructor 1 with (wf:=wf); et; ss.
     econs; ss. init. unfold ccall.
-    harg_tac. des; clarify. unfold fF, ccall. anytac. ss.
+    harg_tac. iRefresh. iDestruct PRE. des; clarify. unfold fF, ccall. anytac. ss.
     steps. astart 10. destruct (dec (Z.of_nat x) 0%Z).
     - destruct x; ss. astop.
       force_l. eexists. hret_tac (@URA.unit Σ) (@URA.unit Σ).
-      { esplits; eauto. }
+      { iRefresh. iSplitP; ss. }
       { split; auto. }
     - destruct x; [ss|]. rewrite Nat2Z.inj_succ. steps.
       acall_tac x (ord_pure x) (@URA.unit Σ) (@URA.unit Σ) (@URA.unit Σ).
       { replace (Z.succ (Z.of_nat x) - 1)%Z with (Z.of_nat x) by lia. ss. }
       { splits; ss. auto with ord_step. }
       { split; auto. }
-      des. subst. anytac. asimpl. steps. astop.
+      iDestruct POST. des. subst. anytac. asimpl. steps. astop.
       force_l. eexists. hret_tac (@URA.unit Σ) (@URA.unit Σ).
-      { splits; auto. unfold sum. splits; auto. ss. repeat f_equal. lia. }
+      { iRefresh. iSplitP; ss. splits; auto. unfold sum. splits; auto. ss. repeat f_equal. lia. }
       { split; ss. }
   Qed.
 
