theories/Logic.v
@@ -1,12 +1,6 @@
 Require Import Coqlib.
-Require Import ITreelib.
 Require Import Universe.
-Require Import STS.
-Require Import Behavior.
-Require Import ModSem.
-Require Import Skeleton.
 Require Import PCM.
-Require Import HoareDef.
 
 Generalizable Variables E R A B C X Y Σ.
 
